rev Data/Array rev Data/List

GMLInit/Data/Array/Basic.lean
@@ -1,7 +1,13 @@
+import GMLInit.Data.BEq
 import GMLInit.Data.Fin
 import GMLInit.Data.List.Basic
 
 namespace Array
+
+protected theorem eq : {as bs : Array α} → as.data = bs.data → as = bs
+| ⟨_⟩, ⟨_⟩, rfl => rfl
+
+@[simp] theorem data_nil {α} : #[].data = ([] : List α) := rfl
 
 /- set -/
 
@@ -112,5 +118,338 @@ theorem get_del (as : Array α) (k : Fin as.size) (i : Nat) (hi : i < (as.del k)
   rw [get_swap]
   rw [if_neg hi']
   rfl
+
+section foldlM
+variable {m} [Monad m] (f : β → α → m β) (b : β)
+
+theorem foldlM_stop (as : Array α) (stop : Nat) (hstop : stop ≤ as.size) : as.foldlM f b stop stop = pure b := by
+  simp only [Array.foldlM]
+  rw [dif_pos hstop]
+  rw [Array.foldlM.loop]
+  rw [dif_neg (by irreflexivity)]
+
+theorem foldlM_step (as : Array α) (start stop : Nat) (hstart : start < stop) (hstop : stop ≤ as.size) :
+  have : start < as.size := Nat.lt_of_lt_of_le hstart hstop
+  as.foldlM f b start stop = f b as[start] >>= fun b => as.foldlM f b (start+1) stop := by
+  simp only [Array.foldlM]
+  rw [dif_pos hstop]
+  rw [Array.foldlM.loop]
+  rw [dif_pos hstart]
+  split
+  next heq =>
+    absurd heq
+    apply Nat.sub_ne_zero_of_lt hstart
+  next heq =>
+    simp
+    congr
+    funext b
+    rw [dif_pos hstop]
+    rw [Nat.sub_succ, heq, Nat.pred_succ]
+
+end foldlM
+
+section foldl
+variable (f : β → α → β) (b : β)
+
+theorem foldl_stop (as : Array α) (stop : Nat) (hstop : stop ≤ as.size) : as.foldl f b stop stop = b := by
+  apply foldlM_stop; assumption
+
+theorem foldl_step (as : Array α) (start stop : Nat) (hstart : start < stop) (hstop : stop ≤ as.size) :
+  have : start < as.size := Nat.lt_of_lt_of_le hstart hstop
+  as.foldl f b start stop = as.foldl f (f b as[start]) (start+1) stop := by
+  apply foldlM_step; assumption; assumption
+
+variable (h : α → α → α) [Lean.IsAssociative h]
+
+theorem foldl_assoc (as : Array α) (b c : α) (start stop : Nat) (hstart : start ≤ stop) (hstop : stop ≤ as.size) :
+  as.foldl h (h b c) start stop = h b (as.foldl h c start stop) := by
+  by_cases start = stop with
+  | isTrue heq =>
+    cases heq
+    rw [foldl_stop] <;> try (exact hstop)
+    rw [foldl_stop]; exact hstop
+  | isFalse hne =>
+    have hstart' : start < stop := Nat.lt_of_le_of_ne hstart hne
+    have : start < as.size := Nat.lt_of_lt_of_le hstart' hstop
+    rw [foldl_step h (h b c)] <;> try (first | exact hstop | exact hstart')
+    rw [foldl_step h c] <;> try (first | exact hstop | exact hstart')
+    rw [Lean.IsAssociative.assoc (op:=h)]
+    rw [foldl_assoc as b (h c as[start]) (start+1) stop hstart' hstop]
+termination_by foldl_assoc => stop - start
+
+end foldl
+
+section foldrM
+variable {m} [Monad m] (f : α → β → m β) (b : β)
+
+theorem foldrM_stop (as : Array α) (stop : Nat) (hstop : stop ≤ as.size) : as.foldrM f b stop stop = pure b := by
+  simp only [Array.foldrM]
+  rw [dif_pos hstop]
+  rw [if_neg (by irreflexivity)]
+
+theorem foldrM_step (as : Array α) (start stop : Nat) (hstop : stop ≤ start) (hstart : start < as.size) :
+  as.foldrM f b (start+1) stop = f as[start] b >>= fun b => as.foldrM f b start stop := by
+  simp only [Array.foldrM]
+  rw [dif_pos (Nat.succ_le_of_lt hstart)]
+  rw [if_pos (Nat.lt_succ_of_le hstop)]
+  simp only [foldrM.fold]
+  split
+  next heq =>
+    absurd (eq_of_beq heq)
+    apply Nat.ne_of_gt
+    apply Nat.lt_succ_of_le
+    exact hstop
+  next hne =>
+    congr
+    funext b
+    rw [dif_pos (Nat.le_of_lt hstart)]
+    split
+    next => rfl
+    next hge =>
+      have : stop = start := by
+        antisymmetry using LE.le
+        · exact hstop
+        · exact Nat.le_of_not_gt hge
+      simp [this]
+      unfold foldrM.fold
+      rw [BEq.rfl, if_pos rfl]
+
+end foldrM
+
+section foldr
+variable (f : α → β → β) (b : β)
+
+theorem foldr_stop (as : Array α) (stop : Nat) (hstop : stop ≤ as.size) : as.foldr f b stop stop = b := by
+  apply foldrM_stop; assumption
+
+theorem foldr_step (as : Array α) (start stop : Nat) (hstop : stop ≤ start) (hstart : start < as.size) :
+  as.foldr f b (start+1) stop = as.foldr f (f as[start] b) start stop := by
+  apply foldrM_step; assumption
+
+end foldr
+
+section append
+
+theorem size_append_aux {as bs : Array α} (start stop : Nat) (hstart : start ≤ stop) (hstop : stop ≤ bs.size) :
+  (foldl push as bs start stop).size = as.size + (stop - start) := by
+  by_cases start = stop with
+  | isTrue heq =>
+    rw [heq]
+    rw [foldl_stop]
+    rw [Nat.sub_self]
+    rw [Nat.add_zero]
+    exact hstop
+  | isFalse hne =>
+    have hstart' : start < stop := Nat.lt_of_le_of_ne hstart hne
+    rw [foldl_step push as bs start stop hstart' hstop]
+    rw [size_append_aux (start+1) stop hstart' hstop]
+    rw [size_push]
+    rw [Nat.sub_succ']
+    rw [Nat.add_assoc]
+    congr
+    rw [Nat.add_comm]
+    have : 1 ≤ stop - start := by
+      rw [Nat.le_sub_iff_add_le hstart]
+      rw [Nat.add_comm]
+      exact hstart'
+    rw [Nat.sub_add_cancel this]
+termination_by size_append_aux => stop - start
+
+theorem get_append_aux_lo {as bs : Array α} (start stop i : Nat) (hstart : start ≤ stop) (hstop : stop ≤ bs.size) (hi : i < as.size)
+  (h : i < (foldl push as bs start stop).size := by simp_arith [*]) :
+  (foldl push as bs start stop)[i] = as[i] := by
+  simp only [autoParam] at h
+  by_cases start = stop with
+  | isTrue heq =>
+    congr
+    rw [heq]
+    rw [foldl_stop]
+    exact hstop
+  | isFalse hne =>
+    have hstart' : start < stop := Nat.lt_of_le_of_ne hstart hne
+    have : start < bs.size := Nat.lt_of_lt_of_le hstart' hstop
+    have : i < (foldl push (as.push bs[start]) bs (start+1) stop).size := by
+      rw [←foldl_step]
+      exact h
+      exact hstart'
+      exact hstop
+    transitivity (foldl push (as.push bs[start]) bs (start+1) stop)[i]
+    · congr 1
+      rw [foldl_step]
+      exact hstart'
+      exact hstop
+    · rw [get_append_aux_lo (start+1) stop i hstart' hstop]
+      rw [get_push_lt]
+termination_by get_append_aux_lo => stop - start
+
+theorem get_append_aux_hi {as bs : Array α} (start stop i : Nat) (hstart : start ≤ stop) (hstop : stop ≤ bs.size) (hi : i < stop - start)
+  (ha : as.size + i < (foldl push as bs start stop).size := by simp_arith [*])
+  (hb : start + i < bs.size := by simp_arith [*]):
+  (foldl push as bs start stop)[as.size + i] = bs[start + i] := by
+  simp only [autoParam] at ha hb
+  by_cases start = stop with
+  | isTrue heq =>
+    rw [heq, Nat.sub_self] at hi
+    contradiction
+  | isFalse hne =>
+    have hstart' : start < stop := Nat.lt_of_le_of_ne hstart hne
+    have : start < bs.size := Nat.lt_of_lt_of_le hstart' hstop
+    have : as.size + i < (foldl push (as.push bs[start]) bs (start+1) stop).size := by
+      rw [size_append_aux (start+1) stop (Nat.succ_le_of_lt hstart') hstop]
+      rw [size_push]
+      rw [Nat.add_assoc]
+      apply Nat.add_lt_add_left
+      rw [Nat.add_comm]
+      rw [Nat.sub_succ']
+      rw [Nat.sub_add_cancel]
+      exact hi
+      rw [Nat.le_sub_iff_add_le hstart]
+      rw [Nat.add_comm]
+      exact Nat.succ_le_of_lt hstart'
+    transitivity (foldl push (as.push bs[start]) bs (start+1) stop)[as.size + i]
+    · congr 1
+      rw [foldl_step]
+      exact hstart'
+      exact hstop
+    · match i with
+      | 0 =>
+        transitivity (as.push bs[start])[as.size]
+        · have h : as.size < (as.push bs[start]).size := by simp; done
+          exact get_append_aux_lo (start+1) stop as.size (Nat.succ_le_of_lt hstart') hstop h _
+        · rw [get_push_eq]; rfl
+      | i+1 =>
+        have : (as.push bs[start]).size + i < (foldl push (as.push bs[start]) bs (start+1) stop).size := by
+          rw [size_append_aux (start+1) stop (Nat.succ_le_of_lt hstart') hstop]
+          rw [size_push]
+          apply Nat.add_lt_add_left
+          rw [Nat.sub_succ']
+          rw [Nat.lt_sub_iff_add_lt]
+          exact hi
+        transitivity (foldl push (as.push bs[start]) bs (start+1) stop)[(as.push bs[start]).size + i]
+        · congr 1
+          rw [size_push]
+          rw [Nat.add_right_comm, Nat.add_assoc]
+        · have hi' : i < stop - (start+1) := by
+            rw [Nat.sub_succ']
+            rw [Nat.lt_sub_iff_add_lt]
+            exact hi
+          have : start + 1 + i < bs.size := by rw [Nat.add_assoc, Nat.add_comm 1]; exact hb
+          rw [get_append_aux_hi (start+1) stop i (Nat.succ_le_of_lt hstart') hstop hi' _ _]
+          congr 1
+          rw [Nat.add_right_comm, Nat.add_assoc]
+          assumption
+
+theorem data_append_aux {as bs : Array α} (start stop : Nat) (hstart : start ≤ stop) (hstop : stop ≤ bs.size) :
+  (foldl push as bs start stop).data = as.data ++ bs.data.extract start stop := by
+  by_cases start = stop with
+  | isTrue heq =>
+    cases heq
+    rw [foldl_stop] <;> try assumption
+    rw [List.extract_stop]
+    rw [List.append_nil]
+  | isFalse hne =>
+    have hstart' : start < stop := Nat.lt_of_le_of_ne hstart hne
+    have : start < bs.size := Nat.lt_of_lt_of_le hstart' hstop
+    rw [foldl_step] <;> try assumption
+    rw [List.extract_step]
+    rw [data_append_aux (start+1) stop] <;> try assumption
+    rw [push_data]
+    rw [getElem_eq_data_get]
+    rw [List.append_assoc]
+    rw [List.singleton_append]
+termination_by data_append_aux => stop - start
+
+theorem size_append (as bs : Array α) : (as ++ bs).size = as.size + bs.size :=
+  size_append_aux 0 bs.size (Nat.zero_le _) (Nat.le_refl _)
+
+theorem get_append_left {as bs : Array α} (i : Nat) (hi : i < as.size) :
+  have : i < (as ++ bs).size := size_append as bs ▸ Nat.lt_add_right _ _ _ hi
+  (as ++ bs)[i] = as[i] :=
+  get_append_aux_lo 0 bs.size i (Nat.zero_le _) (Nat.le_refl _) hi _
+
+theorem get_append_right {as bs : Array α} (i : Nat) (hi : i < bs.size) :
+  have : as.size + i < (as ++ bs).size := size_append as bs ▸ Nat.add_lt_add_left hi as.size
+  (as ++ bs)[as.size + i] = bs[i] := by
+  simp only [HAppend.hAppend, Append.append, Array.append]
+  rw [get_append_aux_hi 0 bs.size i (Nat.zero_le _) (Nat.le_refl _) hi _ _]
+  congr
+  rw [Nat.zero_add]
+  rw [Nat.zero_add]
+  exact hi
+
+theorem data_append {as bs : Array α} : (as ++ bs).data = as.data ++ bs.data := by
+  simp only [HAppend.hAppend, Append.append, Array.append]
+  rw [data_append_aux 0 bs.size (Nat.zero_le _) (Nat.le_refl _)]
+  rw [List.extract_all]; rfl
+
+theorem nil_append (as : Array α) : #[] ++ as = as := by
+  apply Array.eq
+  repeat rw [data_append]
+  rw [data_nil]
+  exact List.nil_append ..
+
+theorem append_nil (as : Array α) : as ++ #[] = as := by
+  apply Array.eq
+  repeat rw [data_append]
+  rw [data_nil]
+  exact List.append_nil ..
+
+theorem append_assoc (as bs cs : Array α) : (as ++ bs) ++ cs = as ++ (bs ++ cs) := by
+  apply Array.eq
+  repeat rw [data_append]
+  exact List.append_assoc ..
+
+end append
+
+section sum
+
+local instance : Lean.IsAssociative (α:=Nat) (.+.) where
+  assoc := Nat.add_assoc
+
+def sum (ns : Array Nat) (start := 0) (stop := ns.size) : Nat :=
+  ns.foldl (.+.) 0 start stop
+
+theorem sum_stop (ns : Array Nat) (stop : Nat) (hstop : stop ≤ ns.size) :
+  ns.sum stop stop = 0 := by
+  simp only [sum]
+  rw [foldl_stop]
+  exact hstop
+
+theorem sum_step (ns : Array Nat) (start stop : Nat) (hstart : start < stop) (hstop : stop ≤ ns.size) :
+  have : start < ns.size := Nat.lt_of_lt_of_le hstart hstop
+  ns.sum start stop = ns[start] + ns.sum (start+1) stop := by
+  have : start < ns.size := Nat.lt_of_lt_of_le hstart hstop
+  simp only [sum]
+  rw [foldl_step] <;> try assumption
+  rw [Nat.add_comm 0 ns[start]]
+  rw [ns.foldl_assoc (.+.) ns[start] 0 (start+1) stop (Nat.succ_le_of_lt hstart) hstop]
+
+end sum
+
+section join
+
+local instance : Lean.IsAssociative (α:=Array α) (.++.) where
+  assoc := append_assoc
+
+def join (as : Array (Array α)) (start := 0) (stop := as.size) : Array α :=
+  as.foldl (.++.) #[] start stop
+
+def join_stop (as : Array (Array α)) (stop : Nat) (hstop : stop ≤ as.size) :
+  as.join stop stop = #[] := by
+  simp only [join]
+  rw [foldl_stop]
+  exact hstop
+
+def join_step (as : Array (Array α)) (start stop : Nat) (hstart : start < stop) (hstop : stop ≤ as.size) :
+  have : start < as.size := Nat.lt_of_lt_of_le hstart hstop
+  as.join start stop = as[start] ++ as.join (start+1) stop := by
+  have : start < as.size := Nat.lt_of_lt_of_le hstart hstop
+  simp only [join]
+  rw [foldl_step] <;> try assumption
+  transitivity (foldl (.++.) (as[start] ++ #[]) as (start+1) stop)
+  · rw [nil_append, append_nil]
+  · rw [foldl_assoc] <;> assumption
+
+end join
 
 end Array
